test/UnfoldTest.v
@@ -1,0 +1,87 @@
+(*We test (non-recursive) function unfolding.
+  We do not yet have a tactic for predicate unfolding, though
+  it would be the exact same*)
+Require Import Task.
+Require Import Theory.
+Require Import Typechecker.
+Require Import Tactics.
+From mathcomp Require Import all_ssreflect.
+Set Bullet Behavior "Strict Subproofs".
+Require Import Coq.QArith.QArith_base.
+
+(*The rational 1/2*)
+Definition half : Q := 1 # 2.
+(*The int 5*)
+Definition five : Z := 5.
+
+(*Test: if we have function fst (x: 'a) (y: 'b) : 'a = x
+  and function snd (x: 'a) (y: 'b) : 'b = y,
+  then fst (0, q0)*)
+Module FunUnfold.
+
+Local Open Scope string_scope.
+
+Definition a : vty := vty_var "a".
+Definition b: vty := vty_var "b".
+Definition x : vsymbol := ("x", a).
+Definition y: vsymbol := ("y", b).
+
+
+(*We need an ADT for the termination check*)
+Definition tunit_ts : typesym :=
+  mk_ts "unit" nil.
+Definition tunit_ty : vty := vty_cons tunit_ts nil.
+Definition tt_fs : funsym :=
+  funsym_noty "tt" nil tunit_ty.
+Definition tunit : alg_datatype :=
+    alg_def tunit_ts (ne_hd tt_fs).
+Definition munit : mut_adt :=
+  mk_mut [tunit] nil erefl.
+  Definition u: vsymbol := ("u", tunit_ty).
+Definition tt_t : term :=
+  Tfun tt_fs nil nil.
+
+Definition fst_fs : funsym :=
+  funsym_noty "fst" [tunit_ty; a; b] a.
+Definition snd_fs : funsym :=
+  funsym_noty "snd" [tunit_ty; a; b] b.
+
+Definition fst_fun : funpred_def :=
+  fun_def fst_fs [u; x;y] (Tvar x).
+Definition snd_fun : funpred_def :=
+  fun_def snd_fs [u; x;y] (Tvar y).
+
+Definition thalf : term := Tconst (ConstReal half).
+Definition tfive : term := Tconst (ConstInt five).
+
+Definition unfold_theory : theory :=
+  rev [
+  tdef (datatype_def munit);  
+  tdef (recursive_def [fst_fun]);
+   tdef (recursive_def [snd_fun]);
+   tprop Pgoal "fst_lemma" (Feq vty_int 
+    (Tfun fst_fs [vty_int; vty_real] [tt_t; tfive; thalf])
+    tfive);
+   tprop Pgoal "snd_lemma" (Feq vty_real
+    (Tfun snd_fs [vty_int; vty_real] [tt_t; tfive; thalf])
+    thalf)].
+
+Lemma unfold_theory_typed : typed_theory unfold_theory.
+Proof.
+  check_theory.
+Qed.
+
+Ltac extra_simpl ::= fold thalf; fold tfive.
+
+Lemma unfold_theory_valid: valid_theory unfold_theory.
+Proof.
+  simpl. split_all; auto.
+  - wstart. 
+    wunfold snd_fs.
+    wreflexivity.
+  - wstart.
+    wunfold fst_fs.
+    wreflexivity.
+Qed.
+
+End FunUnfold.
